Derive a spec for bellman-ford using a within filter

examples/proofs/Bellman_ford_proof.v
@@ -170,3 +170,49 @@ Proof.
   { ultimately_greater. } { monotonic. }
   simpl. eapply dominated_mul_cst_l_2_2. reflexivity.
 Qed.
+
+Definition domain := (fun '(n,m) => m <= n ^ 2).
+
+Lemma domain_often :
+  often
+    (product_filterType Z_filterType Z_filterType)
+    domain.
+Proof.
+  unfold often. simpl. intros Q U.
+  rewrite productP in U. destruct U as (P1 & P2 & U1 & U2 & H).
+  rewrite (ZP_ultimately (ultimately_ge_Z 1)) in U1.
+  rewrite (ZP_ultimately (ultimately_ge_Z 1)) in U2.
+  destruct U2 as (m0 & M0 & Hm0). destruct U1 as (n0 & N0 & Hn0).
+  exists (Z.max n0 m0, (Z.max n0 m0) ^ 2).
+  split; swap 1 2.
+  - apply H. apply Hn0. math_lia. apply Hm0. math_nia.
+  - unfold domain. reflexivity.
+Qed.
+
+Lemma bellman_ford2_spec_derived :
+  specO
+    (within_filterType
+      (product_filterType Z_filterType Z_filterType)
+      domain
+      domain_often)
+    eq (* TODO *)
+    (fun cost =>
+      forall (inf : int) t (edges : list (int * int * int)%type) (nb_nodes : int),
+        1 <= nb_nodes ->
+        app bellman_ford2 [inf t nb_nodes]
+        PRE (\$ (cost (nb_nodes, LibListZ.length edges)) \* t ~> Array edges)
+        POST (fun (_: array int) => t ~> Array edges))
+    (fun '(n,m) => n ^ 3).
+Proof.
+  econstructor; try apply bellman_ford2_spec.
+  eapply dominated_transitive.
+  { destruct (cost_dominated bellman_ford2_spec) as [c U].
+    exists c. applys within_finer U. }
+  { exists 1. rewrite withinP.
+    rewrite productP. do 2 exists (fun x => 0 <= x).
+    splits; try apply ultimately_ge_Z.
+    intros n m N M D. unfold domain in D.
+    rewrite Z.abs_eq; [| math_nia].
+    rewrite Z.abs_eq; swap 1 2. apply~ Z.pow_nonneg.
+    rewrite D. math_nia. }
+Qed.
